src/SizeClass.fst
@@ -134,60 +134,8 @@ let allocate_size_class_sl_lemma2
   )
   = ()
 
+open MiscArith
 #push-options "--fuel 0 --ifuel 0"
-let mod_arith_lemma
-  (n: nat) (k1 k2: pos)
-  : Lemma
-  (requires
-    k1 % k2 == 0 /\
-    k2 <= k1
-  )
-  (ensures
-    (n % k1) % k2 == n % k2
-  )
-  =
-  calc (==) {
-    ((n / k1) * k1) % k2;
-    == { Math.Lemmas.lemma_mod_mul_distr_r (n / k1) k1 k2 }
-    ((n / k1) * (k1 % k2)) % k2;
-    == { () }
-    0;
-  };
-  assert (((n / k1) * k1) % k2 == 0);
-  calc (==) {
-    (n % k1) % k2;
-    == { FStar.Math.Lemmas.euclidean_division_definition n k1 }
-    (n - (n / k1) * k1) % k2;
-    == { FStar.Math.Lemmas.lemma_mod_sub_distr n ((n / k1) * k1) k2 }
-    (n - ((n / k1) * k1) % k2) % k2;
-    == { () }
-    n % k2;
-  }
-
-let lemma_mod_plus2 (a k: int) (n: pos)
-  : Lemma
-  (requires
-    k % n == 0
-  )
-  (ensures
-    (a + k) % n == a % n
-  )
-  =
-  assert (k == k/n*n);
-  let k' = k/n in
-  Math.Lemmas.lemma_mod_plus a k' n
-
-let lemma_mod_mul2 (a k: int) (n: pos)
-  : Lemma
-  (requires
-    k % n == 0
-  )
-  (ensures
-    (a * k) % n == 0
-  )
-  =
-  Math.Lemmas.lemma_mod_mul_distr_r a k n
-
 let mod_arith_lemma_applied
   (n: nat) (page_size sc align: pos)
   : Lemma
