lib_misc/MiscArith.fst
@@ -1,0 +1,62 @@
+module MiscArith
+
+#push-options "--fuel 0 --ifuel 0"
+
+open FStar.Mul
+
+//TODO: to be removed
+//let mod_arith_lemma
+//  (n: nat) (k1 k2: pos)
+//  : Lemma
+//  (requires
+//    k1 % k2 == 0 /\
+//    k2 <= k1
+//  )
+//  (ensures
+//    (n % k1) % k2 == n % k2
+//  )
+//  =
+//  calc (==) {
+//    ((n / k1) * k1) % k2;
+//    == { Math.Lemmas.lemma_mod_mul_distr_r (n / k1) k1 k2 }
+//    ((n / k1) * (k1 % k2)) % k2;
+//    == { () }
+//    0;
+//  };
+//  assert (((n / k1) * k1) % k2 == 0);
+//  calc (==) {
+//    (n % k1) % k2;
+//    == { FStar.Math.Lemmas.euclidean_division_definition n k1 }
+//    (n - (n / k1) * k1) % k2;
+//    == { FStar.Math.Lemmas.lemma_mod_sub_distr n ((n / k1) * k1) k2 }
+//    (n - ((n / k1) * k1) % k2) % k2;
+//    == { () }
+//    n % k2;
+//  }
+
+let lemma_mod_plus2 (a k: int) (n: pos)
+  : Lemma
+  (requires
+    k % n == 0
+  )
+  (ensures
+    (a + k) % n == a % n
+  )
+  =
+  assert (k == k/n*n);
+  let k' = k/n in
+  Math.Lemmas.lemma_mod_plus a k' n
+
+let lemma_mod_mul2 (a k: int) (n: pos)
+  : Lemma
+  (requires
+    k % n == 0
+  )
+  (ensures
+    (a * k) % n == 0
+  )
+  =
+  Math.Lemmas.lemma_mod_mul_distr_r a k n
+
+let lemma_mul_le (a b c c':nat) : Lemma (requires c <= c') (ensures a * b * c <= a * b * c')
+  = ()
